minor reifier changes

theories/gitree/greifiers.v
@@ -116,7 +116,7 @@ Section greifiers.
   Program Definition gReifiers_re {n} (rs : gReifiers n) {X} `{!Cofe X}
     (op : opid (gReifiers_ops rs)) :
     (Ins (gReifiers_ops rs op) ♯ X) * (gReifiers_state rs ♯ X) * ((Outs (gReifiers_ops rs op) ♯ X) -n> laterO X) -n>
-      optionO ((Outs (gReifiers_ops rs op) ♯ X) * (gReifiers_state rs ♯ X))
+      optionO (laterO X * (gReifiers_state rs ♯ X))
     :=  λne xst,
       let  i := projT1 op in
       let op' := projT2 op in
@@ -137,104 +137,127 @@ Section greifiers.
        sReifier_re := @gReifiers_re n rs;
     |}.
 
-  (* Lemma gReifiers_re_idx {n}  (i : fin n) (rs : gReifiers n) *)
-  (*   {X} `{!Cofe X} (op : opid (sReifier_ops (rs !!! i))) *)
-  (*   (x : Ins (sReifier_ops _ op) ♯ X) *)
-  (*   (σ : sReifier_state (rs !!! i) ♯ X) (rest : gState_rest i rs ♯ X) : *)
-  (*   gReifiers_re rs (existT i op) (x, gState_recomp rest σ) ≡ *)
-  (*     optionO_map (prodO_map idfun (gState_recomp rest)) *)
-  (*          (sReifier_re (rs !!! i) op (x,σ)). *)
-  (* Proof. *)
-  (*   unfold gReifiers_re. cbn-[prodO_map optionO_map]. *)
-  (*   f_equiv; last repeat f_equiv. *)
-  (*   - eapply optionO_map_proper. *)
-  (*     intros [x1 x2]; simpl. f_equiv. *)
-  (*     f_equiv. f_equiv. *)
-  (*     rewrite gState_decomp_recomp//. *)
-  (*   - rewrite gState_decomp_recomp//. *)
-  (* Qed. *)
+  Lemma gReifiers_re_idx {n} (i : fin n) (rs : gReifiers n)
+    {X} `{!Cofe X} (op : opid (sReifier_ops (rs !!! i)))
+    (x : Ins (sReifier_ops _ op) ♯ X)
+    (σ : sReifier_state (rs !!! i) ♯ X)
+    (κ : (Outs (sReifier_ops (rs !!! i) op) ♯ X -n> laterO X))
+    (rest : gState_rest i rs ♯ X) :
+    gReifiers_re rs (existT i op) (x, gState_recomp rest σ, κ) ≡
+      optionO_map (prodO_map idfun (gState_recomp rest))
+      (sReifier_re (rs !!! i) op (x, σ, κ)).
+  Proof.
+    unfold gReifiers_re. cbn-[prodO_map optionO_map].
+    f_equiv; last repeat f_equiv.
+    - eapply optionO_map_proper.
+      intros [x1 x2]; simpl. f_equiv.
+      f_equiv. f_equiv.
+      rewrite gState_decomp_recomp//.
+    - rewrite gState_decomp_recomp//.
+  Qed.
 
-  (* Class subReifier {n} (r : sReifier) (rs : gReifiers n) := *)
-  (*   { sR_idx : fin n; *)
-  (*     sR_ops :: subEff (sReifier_ops r) (sReifier_ops (rs !!! sR_idx)); *)
-  (*     sR_state  {X} `{!Cofe X} : *)
-  (*       sReifier_state r ♯ X ≃ sReifier_state (rs !!! sR_idx) ♯ X; *)
-  (*     sR_re (m : nat) {X} `{!Cofe X} (op : opid (sReifier_ops r)) *)
-  (*       (x : Ins (sReifier_ops _ op) ♯ X) *)
-  (*       (y : Outs (sReifier_ops _ op) ♯ X) *)
-  (*       (s1 s2 : sReifier_state r ♯ X) *)
-  (*       (k : (Outs (sReifier_ops _ op) ♯ X -n> laterO X)) : *)
-  (*       sReifier_re r op (x, s1, k) ≡{m}≡ Some (y, s2) → *)
-  (*       sReifier_re (rs !!! sR_idx) (subEff_opid op) *)
-  (*         (subEff_ins x, sR_state s1, _) ≡{m}≡ *)
-  (*         Some (subEff_outs y, sR_state s2) }. *)
+  Class subReifier {n} (r : sReifier) (rs : gReifiers n) :=
+    { sR_idx : fin n;
+      sR_ops :: subEff (sReifier_ops r) (sReifier_ops (rs !!! sR_idx));
+      sR_state {X} `{!Cofe X} :
+      sReifier_state r ♯ X ≃ sReifier_state (rs !!! sR_idx) ♯ X;
+      sR_re (m : nat) {X} `{!Cofe X} (op : opid (sReifier_ops r))
+        (x : Ins (sReifier_ops r op) ♯ X)
+        (y : Outs (sReifier_ops r op) ♯ X)
+        (s1 s2 : sReifier_state r ♯ X)
+        (k : (Outs (sReifier_ops r op) ♯ X -n> laterO X)) :
+      sReifier_re r op (x, s1, k) ≡{m}≡ Some ((prodO_map k idfun (y, s2))) →
+      sReifier_re (rs !!! sR_idx) (subEff_opid op)
+        (subEff_ins x, sR_state s1, ccompose k (subEff_outs ^-1)) ≡{m}≡
+        Some (k y, sR_state s2)
+    }.
 
-  (* #[global] Instance subReifier_here {n} (r : sReifier) (rs : gReifiers n) : *)
-  (*   subReifier r (gReifiers_cons r rs). *)
-  (* Proof. *)
-  (*   simple refine ({| sR_idx := 0%fin |}). *)
-  (*   - simpl. apply subEff_id. *)
-  (*   - simpl. intros. apply iso_ofe_refl. *)
-  (*   - intros X ? op x y s1 s2. *)
-  (*     simpl. eauto. *)
-  (* Defined. *)
-  (* #[global] Instance subReifier_there {n} (r r' : sReifier) (rs : gReifiers n) : *)
-  (*   subReifier r rs → *)
-  (*   subReifier r (gReifiers_cons r' rs). *)
-  (* Proof. *)
-  (*   intros SR. *)
-  (*   simple refine ({| sR_idx := FS sR_idx |}). *)
-  (*   - simpl. intros. apply sR_state. *)
-  (*   - intros X ? op x y s1 s2. *)
-  (*     simpl. apply sR_re. *)
-  (* Defined. *)
+  Lemma ccompose_id_l {A B : ofe} (f : A -n> B) :
+    cid ◎ f ≡ f.
+  Proof.
+    intros x; reflexivity.
+  Qed.
 
-  (* #[local] Definition subR_op {n} {r : sReifier} {rs : gReifiers n} `{!subReifier r rs} : *)
-  (*   opid (sReifier_ops r) → opid (gReifiers_ops rs). *)
-  (* Proof. *)
-  (*   intros op. *)
-  (*   simpl. *)
-  (*   refine (existT sR_idx (subEff_opid op)). *)
-  (* Defined. *)
-  (* #[export] Instance subReifier_subEff {n} {r : sReifier} {rs : gReifiers n} `{!subReifier r rs} : *)
-  (*   subEff (sReifier_ops r) (gReifiers_ops rs). *)
-  (* Proof. *)
-  (*   simple refine {| subEff_opid := subR_op |}. *)
-  (*   - intros op X ?. simpl. *)
-  (*     apply subEff_ins. *)
-  (*   - intros op X ?. simpl. *)
-  (*     apply subEff_outs. *)
-  (* Defined. *)
+  Lemma ccompose_id_r {A B : ofe} (f : A -n> B) :
+    f ◎ cid ≡ f.
+  Proof.
+    intros x; reflexivity.
+  Qed.
 
-  (* Lemma subReifier_reify_idx {n} (r : sReifier) (rs : gReifiers n) *)
-  (*   `{!subReifier r rs} {X} `{!Cofe X} (op : opid (sReifier_ops r)) *)
-  (*   (x : Ins (sReifier_ops _ op) ♯ X) *)
-  (*   (y : Outs (sReifier_ops _ op) ♯ X) *)
-  (*   (s1 s2 : sReifier_state r ♯ X) : *)
-  (*       sReifier_re r op (x, s1) ≡ Some (y, s2) → *)
-  (*       sReifier_re (rs !!! sR_idx) (subEff_opid op) *)
-  (*         (subEff_ins x, sR_state s1) ≡ *)
-  (*         Some (subEff_outs y, sR_state s2). *)
-  (* Proof. *)
-  (*   intros Hx. apply equiv_dist=>m. *)
-  (*   apply sR_re. by apply equiv_dist. *)
-  (* Qed. *)
+  #[global] Instance subReifier_here {n} (r : sReifier) (rs : gReifiers n) :
+    subReifier r (gReifiers_cons r rs).
+  Proof.
+    simple refine ({| sR_idx := 0%fin |}).
+    - simpl. apply subEff_id.
+    - simpl. intros. apply iso_ofe_refl.
+    - intros X ? op x y ? s1 s2 k HEQ; simpl.
+      unfold ofe_iso_1'; simpl.
+      rewrite ccompose_id_r HEQ.
+      reflexivity.
+  Defined.
 
-  (* Lemma subReifier_reify {n} (r : sReifier) *)
-  (*   (rs : gReifiers n) `{!subReifier r rs} {X} `{!Cofe X} *)
-  (*   (op : opid (sReifier_ops r)) *)
-  (*   (x : Ins (sReifier_ops _ op) ♯ X) (y : Outs (sReifier_ops _ op) ♯ X) *)
-  (*   (σ σ' : sReifier_state r ♯ X) (rest : gState_rest sR_idx rs ♯ X) : *)
-  (*   sReifier_re r op (x,σ) ≡ Some (y, σ') → *)
-  (*   gReifiers_re rs (subEff_opid op) *)
-  (*     (subEff_ins x, gState_recomp rest (sR_state σ)) *)
-  (*     ≡ Some (subEff_outs y, gState_recomp rest (sR_state σ')). *)
-  (* Proof. *)
-  (*   intros Hre. *)
-  (*   eapply subReifier_reify_idx in Hre. *)
-  (*   rewrite gReifiers_re_idx//. *)
-  (*   rewrite Hre. simpl. reflexivity. *)
-  (* Qed. *)
+  #[global] Instance subReifier_there {n} (r r' : sReifier) (rs : gReifiers n) :
+    subReifier r rs →
+    subReifier r (gReifiers_cons r' rs).
+  Proof.
+    intros SR.
+    simple refine ({| sR_idx := FS sR_idx |}).
+    - simpl. intros. apply sR_state.
+    - intros X ? op x y s1 s2.
+      simpl. apply sR_re.
+  Defined.
+
+  #[local] Definition subR_op {n} {r : sReifier} {rs : gReifiers n} `{!subReifier r rs} :
+    opid (sReifier_ops r) → opid (gReifiers_ops rs).
+  Proof.
+    intros op.
+    simpl.
+    refine (existT sR_idx (subEff_opid op)).
+  Defined.
+  #[export] Instance subReifier_subEff {n} {r : sReifier} {rs : gReifiers n} `{!subReifier r rs} :
+    subEff (sReifier_ops r) (gReifiers_ops rs).
+  Proof.
+    simple refine {| subEff_opid := subR_op |}.
+    - intros op X ?. simpl.
+      apply subEff_ins.
+    - intros op X ?. simpl.
+      apply subEff_outs.
+  Defined.
+
+  Lemma subReifier_reify_idx {n} (r : sReifier) (rs : gReifiers n)
+    `{!subReifier r rs} {X} `{!Cofe X} (op : opid (sReifier_ops r))
+    (x : Ins (sReifier_ops _ op) ♯ X)
+    (y : Outs (sReifier_ops _ op) ♯ X)
+    (k : (Outs (sReifier_ops r op) ♯ X -n> laterO X))
+    (s1 s2 : sReifier_state r ♯ X) :
+    sReifier_re r op (x, s1, k) ≡ Some ((prodO_map k idfun (y, s2))) →
+      sReifier_re (rs !!! sR_idx) (subEff_opid op)
+        (subEff_ins x, sR_state s1, ccompose k (subEff_outs ^-1)) ≡
+        Some (k y, sR_state s2).
+  Proof.
+    intros Hx. apply equiv_dist=>m.
+    apply sR_re. by apply equiv_dist.
+  Qed.
+
+  Lemma subReifier_reify {n} (r : sReifier)
+    (rs : gReifiers n) `{!subReifier r rs} {X} `{!Cofe X}
+    (op : opid (sReifier_ops r))
+    (x : Ins (sReifier_ops _ op) ♯ X) (y : Outs (sReifier_ops _ op) ♯ X)
+    (k : (Outs (sReifier_ops r op) ♯ X -n> laterO X))
+    (σ σ' : sReifier_state r ♯ X) (rest : gState_rest sR_idx rs ♯ X) :
+    sReifier_re r op (x, σ, k) ≡ Some (prodO_map k idfun (y, σ')) →
+    gReifiers_re rs (subEff_opid op)
+      (subEff_ins x, gState_recomp rest (sR_state σ), ccompose k (subEff_outs ^-1))
+      ≡ Some ((ccompose k (subEff_outs ^-1)) (subEff_outs y), gState_recomp rest (sR_state σ')).
+  Proof.
+    intros Hre.
+    eapply subReifier_reify_idx in Hre.
+    rewrite gReifiers_re_idx//.
+    rewrite Hre. simpl.
+    do 3 f_equiv.
+    unfold ofe_iso_1'; simpl.
+    by rewrite ofe_iso_21.
+  Qed.
 
   (** Lemma for reasoning internally in iProp *)
   Context `{!invGS_gen hlc Σ}.
@@ -243,41 +266,51 @@ Section greifiers.
   Variable (rs : gReifiers sz).
   Notation sr := (gReifiers_sReifier rs).
 
-  Lemma reify_vis_eqI {A} `{!Cofe A} op i k o σ σ' :
-    (gReifiers_re rs op (i,σ,k) ≡ Some (o,σ') ⊢@{iProp} reify sr (Vis op i k : IT _ A) σ ≡ (σ', Tau $ k o))%I.
-  Proof.
-    apply uPred.internal_eq_entails=>m.
-    intros H. apply reify_vis_dist. exact H.
-  Qed.
-  (* Lemma subReifier_reify_idxI (r : sReifier) *)
-  (*   `{!subReifier r rs} {X} `{!Cofe X} (op : opid (sReifier_ops r)) *)
-  (*   (x : Ins (sReifier_ops _ op) ♯ X) *)
-  (*   (y : Outs (sReifier_ops _ op) ♯ X) *)
-  (*   (s1 s2 : sReifier_state r ♯ X) : *)
-  (*       sReifier_re r op (x, s1) ≡ Some (y, s2) ⊢@{iProp} *)
-  (*       sReifier_re (rs !!! sR_idx) (subEff_opid op) *)
-  (*         (subEff_ins x, sR_state s1) ≡ *)
-  (*         Some (subEff_outs y, sR_state s2). *)
+  (* Lemma reify_vis_eqI {A} `{!Cofe A} op i k o σ σ' : *)
+  (*   (gReifiers_re rs op (i, σ, k) ≡ Some (o,σ') ⊢@{iProp} reify sr (Vis op i k : IT _ A) σ ≡ (σ', Tau $ k o))%I. *)
   (* Proof. *)
   (*   apply uPred.internal_eq_entails=>m. *)
-  (*   apply sR_re. *)
+  (*   intros H. apply reify_vis_dist. exact H. *)
   (* Qed. *)
 
-  (* Lemma subReifier_reifyI (r : sReifier) *)
-  (*   `{!subReifier r rs} {X} `{!Cofe X} *)
-  (*   (op : opid (sReifier_ops r)) *)
-  (*   (x : Ins (sReifier_ops _ op) ♯ X) (y : Outs (sReifier_ops _ op) ♯ X) *)
-  (*   (σ σ' : sReifier_state r ♯ X) (rest : gState_rest sR_idx rs ♯ X) : *)
-  (*   sReifier_re r op (x,σ) ≡ Some (y, σ') ⊢@{iProp} *)
-  (*   gReifiers_re rs (subEff_opid op) *)
-  (*     (subEff_ins x, gState_recomp rest (sR_state σ)) *)
-  (*     ≡ Some (subEff_outs y, gState_recomp rest (sR_state σ')). *)
-  (* Proof. *)
-  (*   apply uPred.internal_eq_entails=>m. *)
-  (*   intros He. *)
-  (*   eapply sR_re in He. *)
-  (*   rewrite gReifiers_re_idx//. *)
-  (*   rewrite He. simpl. reflexivity. *)
-  (* Qed. *)
+  Lemma subReifier_reify_idxI (r : sReifier)
+    `{!subReifier r rs} {X} `{!Cofe X} (op : opid (sReifier_ops r))
+    (x : Ins (sReifier_ops _ op) ♯ X)
+    (y : Outs (sReifier_ops _ op) ♯ X)
+    (k : (Outs (sReifier_ops r op) ♯ X -n> laterO X))
+    (s1 s2 : sReifier_state r ♯ X) :
+        sReifier_re r op (x, s1, k) ≡ Some (prodO_map k idfun (y, s2)) ⊢@{iProp}
+        sReifier_re (rs !!! sR_idx) (subEff_opid op)
+          (subEff_ins x, sR_state s1, ccompose k (subEff_outs ^-1)) ≡
+          Some ((ccompose k (subEff_outs ^-1)) (subEff_outs y), sR_state s2).
+  Proof.
+    apply uPred.internal_eq_entails=>m.
+    intros H.
+    rewrite sR_re; last first.
+    - rewrite H.
+      reflexivity.
+    - simpl; rewrite ofe_iso_21.
+      reflexivity.
+  Qed.
+
+  Lemma subReifier_reifyI (r : sReifier)
+    `{!subReifier r rs} {X} `{!Cofe X}
+    (op : opid (sReifier_ops r))
+    (x : Ins (sReifier_ops _ op) ♯ X) (y : Outs (sReifier_ops _ op) ♯ X)
+    (k : (Outs (sReifier_ops r op) ♯ X -n> laterO X))
+    (σ σ' : sReifier_state r ♯ X) (rest : gState_rest sR_idx rs ♯ X) :
+    sReifier_re r op (x,σ, k) ≡ Some (prodO_map k idfun (y, σ')) ⊢@{iProp}
+    gReifiers_re rs (subEff_opid op)
+      (subEff_ins x, gState_recomp rest (sR_state σ), ccompose k (subEff_outs ^-1))
+      ≡ Some ((ccompose k (subEff_outs ^-1)) (subEff_outs y), gState_recomp rest (sR_state σ')).
+  Proof.
+    apply uPred.internal_eq_entails=>m.
+    intros He.
+    eapply sR_re in He.
+    rewrite gReifiers_re_idx//.
+    rewrite He. simpl.
+    rewrite ofe_iso_21.
+    reflexivity.
+  Qed.
 
 End greifiers.
